add fast python

dafny/test.dfy
@@ -113,3 +113,86 @@ predicate sorted(a: array<int>)
        forall j, k :: 0 <= j < k < a.Length ==> a[j] <= a[k]
                       )
 }
+
+method Index(n: int) returns (i: int)
+  requires 1 <= n
+  ensures 0 <= i < n
+{
+  i := n / 2;
+}
+
+method MaxSum(x: int, y: int) returns (s: int, m: int)
+  ensures x <= m && y <= m
+  ensures m == x || m == y
+  ensures s == x + y
+{
+  if x <= y {
+    m := y;
+  } else {
+    m := x;
+  }
+  s := x + y;
+}
+
+method ReconstructFromMaxSum(s: int, m: int) returns (x: int,y: int)
+  requires s <= 2 * m
+  ensures s == x + y
+  ensures (m == x || m == y) && x <= m && y <= m
+{
+  x := m;
+  y := s - m;
+}
+
+method TestMaxSum(x: int, y: int) {
+  var s, m := MaxSum(x, y);
+  var xx, yy := ReconstructFromMaxSum(s, m);
+  assert (x == xx && y == yy) || (x == yy && y == xx);
+}
+
+function Average(a: int, b: int): int {
+  (a + b) / 2
+}
+
+method Triple'(x: int) returns (r: int)
+  ensures Average(r, 3 * x) == 3 * x
+{
+  r := 3 * x + 1;
+}
+
+predicate IsEven(x: int) {
+  x % 2 == 0
+}
+
+method Triple(x: int) returns (r: int)
+  ensures r == 3 * x
+{
+  var y := x * 2;
+  r := x + y;
+  ghost var a, b := DoubleQuadruple(x);
+  assert a <= r <= b || b <= r <= a;
+}
+
+ghost method DoubleQuadruple(x: int) returns (a: int, b: int)
+  ensures a == 2 * x && b == 4 * x
+{
+  a := 2 * x;
+  b := 4 * x;
+}
+
+function F(): int {
+  29
+}
+
+method M2() returns (r: int)
+  ensures r == 29
+{
+  r := 29;
+}
+
+method Caller2()
+{
+  var a := F();
+  var b := M2();
+  assert a == 29;
+  assert b == 29;
+}
